KeyManagement/MessageEq.v
@@ -54,7 +54,7 @@ Inductive message_eq : forall {A B} {t__rw : RealWorld.message.type} {t__iw : Id
     U__rw.(RealWorld.all_ciphers) $? c__id = Some (RealWorld.SigEncCipher k__sig k__enc c) ->
     message_eq c U__rw m__iw U__iw m__expected ch__id ({k__enc} \cup readers) ({k__sig} \cup writers) ->
     (* switch to set of all users that people get removed from *)
-    @message_eq A B t__rw t__iw (RealWorld.SignedCiphertext k__enc k__sig c__id) U__rw m__iw U__iw m__expected ch__id readers writers
+    @message_eq A B t__rw t__iw (RealWorld.SignedCiphertext c__id) U__rw m__iw U__iw m__expected ch__id readers writers
 | SignatureCase : forall {A B t__rw t__iw}
                          (c__id : RealWorld.cipher_id)
                          (m : RealWorld.crypto t__rw) (m__iw m__expected : IdealWorld.message.message t__iw)
@@ -64,7 +64,7 @@ Inductive message_eq : forall {A B} {t__rw : RealWorld.message.type} {t__iw : Id
                          (ch__id : IdealWorld.channel_id),
     U__rw.(RealWorld.all_ciphers) $? c__id = Some (RealWorld.SigCipher k__sig m) ->
     message_eq m U__rw m__iw U__iw m__expected ch__id readers ({k__sig} \cup writers) ->
-    message_eq (RealWorld.Signature m k__sig c__id) U__rw m__iw U__iw m__expected ch__id readers writers.
+    message_eq (RealWorld.Signature m c__id) U__rw m__iw U__iw m__expected ch__id readers writers.
 
 
 (* Definition garbage : option (list RealWorld.key_identifier) * exmsg := *) (*   (None, Exm (RealWorld.Plaintext 0)). *)
